### 1. Infix: ((a + b) + c - d) / (a^2 - b^2)

**Steps**:  
(a + b) → a b +  
(a + b) + c → a b + c +  
(a + b + c) - d → a b + c + d -  
a^2 → a 2 ^  
b^2 → b 2 ^  
(a^2 - b^2) → a 2 ^ b 2 ^ -  
Final: (a + b + c - d) / (a^2 - b^2) → `a b + c + d - a 2 ^ b 2 ^ - /`

---

### 2. Infix: ((sin(x^2) + cos(x^2)) / (a^2 + b^2))

**Steps**:  
x^2 → x 2 ^  
sin(x^2) → x 2 ^ sin  
cos(x^2) → x 2 ^ cos  
sin(x^2) + cos(x^2) → x 2 ^ sin x 2 ^ cos +  
a^2 → a 2 ^  
b^2 → b 2 ^  
a^2 + b^2 → a 2 ^ b 2 ^ +  
Final: (sin(x²) + cos(x²)) / (a² + b²) → `x 2 ^ sin x 2 ^ cos + a 2 ^ b 2 ^ + /`

---

### 3. Infix: {(2b + b*)^*ba + b}

**Steps**:  
2b → 2 b .  
b* → b *  
2b + b* → 2 b . b * .  
(2b + b*)* → 2 b . b * . *  
ba → b a .  
(2b + b*)* ba → 2 b . b * . * b a . .  
+ b → 2 b . b * . * b a . . b +  
Final: `2 b . b * . * b a . . b +`

---

### 4. Infix: (√(b² - 4ac) * (a² + b²))

**Steps**:  
b^2 → b 2 ^  
4ac → 4 a * c *  
b^2 - 4ac → b 2 ^ 4 a * c * -  
√(b^2 - 4ac) → b 2 ^ 4 a * c * - sqrt  
a^2 → a 2 ^  
b^2 → b 2 ^  
a^2 + b^2 → a 2 ^ b 2 ^ +  
Final: √(b² - 4ac) · (a² + b²) → `b 2 ^ 4 a * c * - sqrt a 2 ^ b 2 ^ + *`

---

### 5. Infix: (x^2 + √(x·y)) / (x + y)

**Steps**:  
x^2 → x 2 ^  
x·y → x y *  
√(x·y) → x y * sqrt  
x^2 + √(x·y) → x 2 ^ x y * sqrt +  
x + y → x y +  
Final: (x² + √(xy)) / (x + y) → `x 2 ^ x y * sqrt + x y + /`

---

### 6. Infix: ((x + y)(x - y)) / (x^2 + y^2)

**Steps**:  
x + y → x y +  
x - y → x y -  
(x + y)(x - y) → x y + x y - *  
x^2 → x 2 ^  
y^2 → y 2 ^  
x^2 + y^2 → x 2 ^ y 2 ^ +  
Final: ((x + y)(x - y)) / (x² + y²) → `x y + x y - * x 2 ^ y 2 ^ + /`

---

### 7. Infix: (a + b)^2 - (a - b)^2

**Steps**:  
a + b → a b +  
(a + b)^2 → a b + 2 ^  
a - b → a b -  
(a - b)^2 → a b - 2 ^  
Subtract: → a b + 2 ^ a b - 2 ^ -  
Final: (a + b)^2 - (a - b)^2 → `a b + 2 ^ a b - 2 ^ -`
